theories/MinskyMachines/Util/MMA_pairing.v
@@ -1,0 +1,469 @@
+(*
+  (Alternative) Minsky Machine PACK, UNPACK routines
+  PACK A X Y offset:
+    X := (X+X+1)*(2^Y)
+    Y := 0
+    A := 0 (auxiliary)
+  UNPACK A X Y offset:
+    IF X = (n+n+1)*2^m THEN X := n, Y := m, A := 0 (auxiliary)
+
+  Other subprograms:
+    INC, DEC, JMP, JZ, ZERO, MOVE, MOVE2, HALF
+*)
+
+From Undecidability Require Import
+  MinskyMachines.MM MinskyMachines.MMA.
+
+From Undecidability.Shared.Libs.DLW
+  Require Import Vec.pos Vec.vec Code.sss.
+
+Require Import PeanoNat List Lia Wf_nat.
+Import ListNotations.
+
+Require Import ssreflect ssrbool ssrfun.
+
+Set Default Goal Selector "!".
+
+#[local] Arguments ltof /.
+
+Section FixCounters.
+Context {num_counters : nat}.
+#[local] Notation counter := (pos num_counters).
+#[local] Notation mm_instr := (mm_instr counter).
+#[local] Notation mm_state := (mm_state num_counters).
+
+#[local] Notation "P // s ->> t" := (sss_compute (@mma_sss num_counters) P s t).
+#[local] Notation "P // s -+> t" := (sss_progress (@mma_sss num_counters) P s t).
+#[local] Notation "e #> x" := (vec_pos e x).
+#[local] Notation "e [ v / x ]" := (vec_change e x v).
+
+(* simplify vec_change statements *)
+Definition vec_norm {X Y: counter} (HXY : X <> Y) := (
+  fun v n m => @vec_change_comm nat _ v X Y n m HXY,
+  fun v n m => @vec_change_idem nat _ v X n m,
+  fun v n m => @vec_change_idem nat _ v Y n m,
+  fun v n => @vec_change_neq nat _ v X Y n HXY,
+  fun v n => @vec_change_neq nat _ v Y X n (nesym HXY),
+  fun v n => @vec_change_eq nat _ v X X n erefl,
+  fun v n => @vec_change_eq nat _ v Y Y n erefl,
+  fun v => @vec_change_same nat _ v X,
+  fun v => @vec_change_same nat _ v Y).
+
+Lemma vec_change_same' {X : Type} {n : nat} {v : vec X n} {p : pos n} {x : X} :
+  vec_pos v p = x -> vec_change v p x = v.
+Proof. move=> <-. by apply: vec_change_same. Qed.
+
+(* compose MMA sub-procedures into one MMA procedure *)
+Fixpoint compose (codes : list (nat -> list mm_instr)) (offset : nat) :=
+  match codes with
+  | nil => []
+  | code :: codes => code offset ++ compose codes ((length (code offset))+offset)
+  end.
+
+Fact sss_compute_refl i P (st : mm_state) : (i, P) // st ->> st.
+Proof.  exists 0. by apply: in_sss_steps_0. Qed.
+
+Fact sss_compute_refl' i P (st1 st2 : mm_state) : st1 = st2 -> (i, P) // st1 ->> st2.
+Proof. move=> ->. by apply: sss_compute_refl. Qed.
+
+Lemma subcode_nth_compose i j codes offset :
+  j = length (compose (firstn i codes) offset) ->
+  subcode.subcode (j + offset, nth i codes (fun=> []) (j + offset)) (offset, compose codes offset).
+Proof.
+  move=> -> /=.
+  elim: codes i offset => /=.
+  { rewrite /compose. by move=> [|i] /=; exists nil, nil; rewrite /= Nat.add_0_r. }
+  move=> code codes IH [|i] offset /=.
+  - eexists nil, _. by rewrite /= Nat.add_0_r.
+  - have [l [r [-> Hl]]] := IH i (length (code offset) + offset).
+    eexists (code offset ++ l), _. rewrite !app_length. split; [|lia].
+    rewrite -!app_assoc. do 3 congr app. congr (nth i codes). lia.
+Qed.
+
+(* uses uniform subproc compose structure *)
+Lemma compose_sss_compute_trans {codes : list (nat -> list mm_instr)} {offset} (i : nat) {v st st'} :
+  let j := length (compose (firstn i codes) offset) in
+  (j + offset, (nth i codes (fun _ => [])) (j+offset)) // (j + offset, v) ->> st' ->
+  (offset, compose codes offset) // st' ->> st ->
+  (offset, compose codes offset) // (j + offset, v) ->> st.
+Proof.
+  move=> j H. apply: sss_compute_trans.
+  move: H. apply: subcode_sss_compute. by apply: subcode_nth_compose.
+Qed.
+
+Lemma compose_sss_progress_trans {codes : list (nat -> list mm_instr)} {offset} (i : nat) {v st st'} :
+  let j := length (compose (firstn i codes) offset) in
+  (j + offset, (nth i codes (fun _ => [])) (j+offset)) // (j + offset, v) -+> st' ->
+  (offset, compose codes offset) // st' ->> st ->
+  (offset, compose codes offset) // (j + offset, v) -+> st.
+Proof.
+  move=> j H. apply: sss_progress_compute_trans.
+  move: H. apply: subcode_sss_progress. by apply: subcode_nth_compose.
+Qed.
+
+Lemma compose_sss_compute_length_trans (i : nat) {codes : list (nat -> list mm_instr)} {lengths} {offset} {v st st'} :
+  Forall2 (fun c l => forall j, length (c j) = l) codes lengths ->
+  let j := list_sum (firstn i lengths) in
+  (j + offset, (nth i codes (fun _ => [])) (j+offset)) // (j + offset, v) ->> st' ->
+  (offset, compose codes offset) // st' ->> st ->
+  (offset, compose codes offset) // (j + offset, v) ->> st.
+Proof.
+  move=> Hcl.
+  suff -> : list_sum (firstn i lengths) = length (compose (firstn i codes) offset) by apply: compose_sss_compute_trans.
+  elim: Hcl i offset. { by case. }
+  move=> c l {}codes {}lengths Hcl _ IH [|i] offset. { done. }
+  by rewrite /= app_length -IH Hcl.
+Qed.
+
+Lemma length_compose {codes lengths offset} :
+  Forall2 (fun c l => forall i, length (c i) = l) codes lengths ->
+  length (compose codes offset) = list_sum lengths.
+Proof.
+  move=> H. elim: H offset; [done|].
+  move=> c l {}codes {}lengths Hcl _ IH offset.
+  by rewrite /= app_length Hcl IH.
+Qed.
+
+Arguments compose : simpl never.
+Arguments plus : simpl never.
+
+Definition INC X (offset : nat) : list mm_instr := [INC X].
+
+Definition INC_len := 1.
+
+Lemma INC_spec X v offset :
+  (offset, INC X offset) // (offset, v) ->>
+    (1 + offset, vec_change v X (S (vec_pos v X))).
+Proof.
+  exists 1. apply: in_sss_steps_S; [|by apply: in_sss_steps_0].
+  eexists offset, nil, _, nil, v. rewrite /= Nat.add_0_r.
+  by split; [|split;[|constructor]].
+Qed.
+
+Definition DEC X p (offset : nat) : list mm_instr := [DEC X p].
+
+Definition DEC_len := 1.
+
+Lemma DEC_spec X p v offset :
+  (offset, DEC X p offset) // (offset, v) ->>
+    match vec_pos v X with
+    | 0 => (1 + offset, v)
+    | S x => (p, vec_change v X x)
+    end.
+Proof.
+  exists 1. apply: in_sss_steps_S; [|by apply: in_sss_steps_0].
+  eexists offset, nil, _, nil, v. rewrite /= Nat.add_0_r.
+  split; [done|split;[done|]].
+  case EX: (v#>X) => [|n]; by constructor.
+Qed.
+
+(* jump to address p; A is auxiliary *)
+Definition JMP_codes (A : counter) (p : nat) (offset : nat) : list (nat -> list mm_instr) :=
+  INC A ::
+  DEC A p :: [].
+
+Definition JMP A p (offset : nat) := compose (JMP_codes A p offset) offset.
+
+Definition JMP_len := INC_len+DEC_len.
+
+Lemma JMP_spec A p v offset :
+  (offset, JMP A p offset) // (offset, v) ->> (p, v).
+Proof.
+  rewrite /=. apply: (compose_sss_compute_trans 0). { by apply: INC_spec. }
+  rewrite /=. apply: (compose_sss_compute_trans 1). { by apply: DEC_spec. }
+  rewrite /= (vec_change_eq _ _ erefl) vec_change_idem vec_change_same.
+  by apply sss_compute_refl.
+Qed.
+
+(* IF X = 0 then GOTO p else continue *)
+Definition JZ_codes (X: counter) (p: nat) (offset: nat) : list (nat -> list mm_instr) :=
+  DEC X ((DEC_len+JMP_len)+offset) ::
+  JMP X p ::
+  INC X :: [].
+
+Definition JZ (X: counter) (p: nat) (offset: nat) := compose (JZ_codes X p offset) offset.
+
+Definition JZ_len := DEC_len+JMP_len+INC_len.
+
+Lemma JZ_spec X p v offset :
+  (offset, JZ X p offset) // (offset, v) ->> (if vec_pos v X is 0 then p else JZ_len+offset, v).
+Proof.
+  case EX: (vec_pos v X) => [|n].
+  - apply: (compose_sss_compute_trans 0). { by apply: DEC_spec. }
+    rewrite EX. apply: (compose_sss_compute_trans 1). { by apply: JMP_spec. }
+    by apply: sss_compute_refl.
+  - apply: (compose_sss_compute_trans 0). { by apply: DEC_spec. }
+    rewrite EX. apply: (compose_sss_compute_trans 2). { by apply: INC_spec. }
+    apply: sss_compute_refl'. congr pair.
+    by rewrite vec_change_idem vec_change_eq // vec_change_same'.
+Qed.
+
+(* X := 0 *)
+Definition ZERO_codes (X: counter) (offset: nat) : list (nat -> list mm_instr) :=
+  DEC X (offset) :: [].
+
+Definition ZERO (X: counter) (offset: nat) := compose (ZERO_codes X offset) offset.
+
+Definition ZERO_len := DEC_len.
+
+Lemma ZERO_spec X v offset :
+  (offset, ZERO X offset) // (offset, v) ->>
+  (ZERO_len+offset, vec_change v X 0).
+Proof.
+  elim /(induction_ltof1 _ (fun w => vec_pos w X)) : v => v IH.
+  case EX: (vec_pos v X) => [|n].
+  { apply: (compose_sss_compute_trans 0). { by apply: DEC_spec. }
+    rewrite EX (vec_change_same' EX).
+    by apply: sss_compute_refl. }
+  apply: (compose_sss_compute_trans 0). { by apply: DEC_spec. }
+  rewrite EX. apply: sss_compute_trans. { apply: IH. by rewrite /= EX vec_change_eq. }
+  apply: sss_compute_refl'. by rewrite vec_change_idem.
+Qed.
+
+(* Y := X + Y; X := 0 *)
+Definition MOVE_codes (X: counter) (Y : counter) (offset: nat) : list (nat -> list mm_instr) :=
+    JMP X ((JMP_len + INC_len) + offset) ::
+    INC Y ::
+    DEC X (JMP_len+offset) :: [].
+
+Definition MOVE (X: counter) (Y : counter) (offset: nat) := compose (MOVE_codes X Y offset) offset.
+
+Definition MOVE_len := JMP_len+INC_len+DEC_len.
+
+Lemma MOVE_spec X Y v offset :
+  X <> Y ->
+  (offset, MOVE X Y offset) // (offset, v) ->>
+  (MOVE_len+offset, vec_change (vec_change v Y (vec_pos v Y + vec_pos v X)) X 0).
+Proof.
+  move=> HXY.
+  apply: (compose_sss_compute_trans 0). { by apply: JMP_spec. }
+  elim /(induction_ltof1 _ (fun w => vec_pos w X)) : v => v IH.
+  case EX: (vec_pos v X) => [|n].
+  { apply: (compose_sss_compute_trans 2). { by apply: DEC_spec. }
+    rewrite EX Nat.add_0_r vec_change_same (vec_change_same' EX).
+    by apply: sss_compute_refl. }
+  apply: (compose_sss_compute_trans 2). { by apply: DEC_spec. }
+  rewrite EX. apply: (compose_sss_compute_trans 1). { by apply: INC_spec. }
+  apply: sss_compute_trans. { apply: IH. rewrite /= !(vec_norm HXY) EX. lia. }
+  apply: sss_compute_refl'. by rewrite !(vec_norm HXY) Nat.add_succ_comm.
+Qed.
+
+(* Y := X + Y; Z := X + Z; X := 0 *)
+Definition MOVE2_codes (X Y Z: counter) (offset: nat) : list (nat -> list mm_instr) :=
+    JMP X ((JMP_len+INC_len+INC_len) + offset) ::
+    INC Y ::
+    INC Z ::
+    DEC X (JMP_len+offset) :: [].
+
+Definition MOVE2 (X Y Z: counter) (offset: nat) := compose (MOVE2_codes X Y Z offset) offset.
+
+Definition MOVE2_len := JMP_len+INC_len+INC_len+DEC_len.
+
+Lemma MOVE2_spec X Y Z v offset :
+  X <> Y -> X <> Z ->
+  (offset, MOVE2 X Y Z offset) // (offset, v) ->>
+  (MOVE2_len+offset, vec_change (vec_change (vec_change v Z (vec_pos v Z + vec_pos v X)) Y (vec_pos ((vec_change v Z (vec_pos v Z + vec_pos v X))) Y + vec_pos v X)) X 0).
+Proof.
+  move=> HXY HXZ.
+  apply: (compose_sss_compute_trans 0). { by apply: JMP_spec. }
+  elim /(induction_ltof1 _ (fun w => vec_pos w X)) : v => v IH.
+  case EX: (vec_pos v X) => [|n].
+  { apply: (compose_sss_compute_trans 3). { by apply: DEC_spec. }
+    rewrite EX !Nat.add_0_r !vec_change_same (vec_change_same' EX).
+    by apply: sss_compute_refl. }
+  apply: (compose_sss_compute_trans 3). { by apply: DEC_spec. }
+  rewrite EX. apply: (compose_sss_compute_trans 1). { by apply: INC_spec. }
+  apply: (compose_sss_compute_trans 2). { by apply: INC_spec. }
+  apply: sss_compute_trans. { apply: IH. by rewrite /= !(vec_norm HXY) !(vec_norm HXZ) EX. }
+  apply: sss_compute_refl'. congr pair.
+  have [<-|HYZ] := pos_eq_dec Y Z.
+  - by rewrite !(vec_norm HXY) -!Nat.add_succ_comm.
+  - do 2 rewrite ?(vec_norm HXY) ?(vec_norm HXZ) ?(vec_norm HYZ).
+    by rewrite -!Nat.add_succ_comm.
+Qed.
+
+(* X := (X+X+1)*(2^Y); A := 0; Y := 0
+   A is auxiliary *)
+Definition PACK_codes (A X Y : counter) (offset: nat) : list (nat -> list mm_instr) :=
+  ZERO A :: 
+  MOVE2 X A A ::
+  INC A ::
+  MOVE A X ::
+  JMP A ((ZERO_len+MOVE2_len+INC_len+MOVE_len+JMP_len+MOVE2_len+MOVE_len)+offset) ::
+  MOVE2 X A A ::
+  MOVE A X ::
+  DEC Y ((ZERO_len+MOVE2_len+INC_len+MOVE_len+JMP_len)+offset) :: [].
+
+Definition PACK (A X Y : counter) (offset: nat) := compose (PACK_codes A X Y offset) offset.
+
+Definition PACK_len := ZERO_len+MOVE2_len+INC_len+MOVE_len+JMP_len+MOVE2_len+MOVE_len+DEC_len.
+
+Lemma PACK_len_spec A X Y offset : length (PACK A X Y offset) = PACK_len.
+Proof. done. Qed. 
+
+Lemma PACK_spec A X Y v offset :
+  let x := vec_pos v X in
+  let y := vec_pos v Y in
+  A <> X -> A <> Y -> X <> Y ->
+  (offset, PACK A X Y offset) // (offset, v) ->>
+    (PACK_len+offset, vec_change (vec_change (vec_change v X ((x+x+1) * (2 ^ y))) Y 0) A 0).
+Proof.
+  move=> /= /[dup] HX /nesym H'X /[dup] HY /nesym H'Y HXY.
+  apply: (compose_sss_compute_trans 0). { by apply: ZERO_spec. }
+  apply: (compose_sss_compute_trans 1). { by apply: MOVE2_spec. }
+  apply: (compose_sss_compute_trans 2). { by apply: INC_spec. }
+  apply: (compose_sss_compute_trans 3). { by apply: MOVE_spec. }
+  apply: (compose_sss_compute_trans 4). { by apply: JMP_spec. }
+  rewrite !(vec_norm HX) !Nat.add_0_l.
+  have -> : S ((v#>X) + (v#>X)) = (v#>X) + (v#>X) + 1 by lia.
+  move: ((v#>X) + (v#>X) + 1).
+  elim /(induction_ltof1 _ (fun w => vec_pos w Y)) : v => v IH x.
+  case EY: (vec_pos v Y) => [|n].
+  { apply: (compose_sss_compute_trans 7). { by apply: DEC_spec. }
+    rewrite !(vec_norm HY) !(vec_norm HXY) EY.
+    apply: sss_compute_refl'. congr pair.
+    by rewrite (vec_change_same' EY) /= Nat.mul_1_r. }
+  apply: (compose_sss_compute_trans 7). { by apply: DEC_spec. }
+  rewrite !(vec_norm HY) !(vec_norm HXY) EY.
+  apply: (compose_sss_compute_trans 5). { by apply: MOVE2_spec. }
+  apply: (compose_sss_compute_trans 6). { by apply: MOVE_spec. }
+  do 2 rewrite ?(vec_norm HX) ?(vec_norm HY) ?(vec_norm HXY).
+  apply: sss_compute_trans. { apply: IH. by rewrite /= !(vec_norm HY) EY. }
+  apply: sss_compute_refl'. congr pair.
+  rewrite ?(vec_norm HX) ?(vec_norm HY) ?(vec_norm HXY).
+  rewrite /=. do 2 congr vec_change. lia.
+Qed.
+
+(* X := X/2 if X even goto p else continue *)
+Definition HALF_codes (A X: counter) (p: nat) (offset: nat) : list (nat -> list mm_instr) :=
+  ZERO A ::
+  MOVE X A ::
+  JMP A ((ZERO_len+MOVE_len+JMP_len+INC_len)+offset) ::
+  INC X ::
+  DEC A ((ZERO_len+MOVE_len+JMP_len+INC_len+DEC_len+JMP_len)+offset) ::
+  JMP A p ::
+  DEC A ((ZERO_len+MOVE_len+JMP_len)+offset) :: [].
+
+Definition HALF (A X : counter) (p: nat) (offset: nat) := compose (HALF_codes A X p offset) offset.
+
+Definition HALF_len := ZERO_len+MOVE_len+JMP_len+INC_len+DEC_len+JMP_len+DEC_len.
+
+(* second component is true iff n is even *)
+Fixpoint half (n: nat) : (nat * bool) :=
+  match n with
+  | 0 => (0, true)
+  | S n' => 
+      match half n' with
+      | (m, b) => if b then (m, false) else (S m, true)
+      end
+  end.
+
+Lemma half_spec n :
+  let '(m, b) := half n in n = (if b then 0 else 1) + m + m.
+Proof. elim: n => [|n] /=; [done|case: (half n) => ? []; lia]. Qed.
+
+Lemma half_spec_odd n : half ((n + n + 1) * 2 ^ 0) = (n, false).
+Proof.
+  have := half_spec ((n + n + 1) * 2 ^ 0).
+  case: (half _) => m [] /= *; congr pair; lia.
+Qed.
+
+Lemma half_spec_even n m : half ((n + n + 1) * 2 ^ (S m)) = ((n + n + 1) * 2 ^ m, true).
+Proof.
+  have := half_spec ((n + n + 1) * 2 ^ (S m)).
+  case: (half _) => k []; rewrite /= => ?; congr pair; lia.
+Qed.
+
+Lemma HALF_spec A X p v offset :
+  let x := vec_pos v X in
+  A <> X ->
+  (offset, HALF A X p offset) // (offset, v) ->>
+    let '(m, b) := half x in (if b then p else HALF_len + offset, vec_change (vec_change v X m) A 0).
+Proof.
+  move=> /= /[dup] HX /nesym  H'X.
+  apply: (compose_sss_compute_trans 0). { by apply: ZERO_spec. }
+  apply: (compose_sss_compute_trans 1). { by apply: MOVE_spec. }
+  apply: (compose_sss_compute_trans 2). { by apply: JMP_spec. }
+  rewrite !(vec_norm HX) Nat.add_0_l.
+  suff: forall w, (offset, HALF A X p offset) //
+    (ZERO_len+MOVE_len+JMP_len+INC_len+offset, w) ->>
+    (let '(m, b) := half (vec_pos w A) in (if b then p else HALF_len + offset,
+      vec_change (vec_change w X (vec_pos w X+m)) A 0)).
+  { move=> H. apply: sss_compute_trans; [apply: H|].
+    apply: sss_compute_refl'. rewrite !(vec_norm HX).
+    case: (half _) => [? ?]. by rewrite !(vec_norm HX). }
+  elim /(induction_ltof1 _ (fun w => vec_pos w A)) => {}v IH.
+  case EA: (vec_pos v A) => [|[|n]].
+  - apply: (compose_sss_compute_trans 4). { by apply: DEC_spec. }
+    rewrite EA. apply: (compose_sss_compute_trans 5). { by apply: JMP_spec. }
+    rewrite Nat.add_0_r !(vec_norm HX) (vec_change_same' EA).
+    by apply: sss_compute_refl.
+  - apply: (compose_sss_compute_trans 4). { by apply: DEC_spec. }
+    rewrite EA. apply: (compose_sss_compute_trans 6). { by apply: DEC_spec. }
+    rewrite Nat.add_0_r !(vec_norm HX).
+    by apply: sss_compute_refl.
+  - apply: (compose_sss_compute_trans 4). { by apply: DEC_spec. }
+    rewrite EA. apply: (compose_sss_compute_trans 6). { by apply: DEC_spec. }
+    rewrite vec_change_eq //. apply: (compose_sss_compute_trans 3). { by apply: INC_spec. }
+    apply: sss_compute_trans. { apply: IH. rewrite /= !(vec_norm HX) EA. lia. }
+    apply: sss_compute_refl'. rewrite !(vec_norm HX) /=.
+    case: (half n) => [m []]; congr pair; by rewrite !(vec_norm HX) Nat.add_succ_comm.
+Qed.
+
+(* IF X = (n+n+1)*2^m THEN X := n AND Y := m 
+   A is auxiliary *)
+Definition UNPACK_codes (A X Y: counter) (offset: nat) : list (nat -> list mm_instr) :=
+  JZ X 0 ::
+  ZERO Y ::
+  JMP A ((JZ_len+ZERO_len+JMP_len+INC_len)+offset) ::
+  INC Y ::
+  HALF A X ((JZ_len+ZERO_len+JMP_len)+offset) :: [].
+
+Definition UNPACK (A X Y: counter) (offset: nat) := compose (UNPACK_codes A X Y offset) offset.
+
+Definition UNPACK_len := JZ_len+ZERO_len+JMP_len+INC_len+HALF_len.
+
+Lemma UNPACK_spec {A X Y m n v offset} :
+  let x := vec_pos v X in
+  x = (n + n + 1) * (2 ^ m) ->
+  A <> X -> A <> Y -> X <> Y ->
+  (offset, UNPACK A X Y offset) // (offset, v) ->>
+    (UNPACK_len + offset, vec_change (vec_change (vec_change v X n) Y m) A 0).
+Proof.
+  move=> /= H'X HX HY HXY.
+  apply: (compose_sss_compute_trans 0). { by apply: JZ_spec. }
+  have ->: vec_pos v X = S (vec_pos v X - 1).
+  { rewrite H'X. have := Nat.pow_nonzero 2 m. lia. }
+  apply: (compose_sss_compute_trans 1). { by apply: ZERO_spec. }
+  apply: (compose_sss_compute_trans 2). { by apply: JMP_spec. }
+  suff: forall w, vec_pos w X = (n + n + 1) * 2 ^ m ->
+    (offset, UNPACK A X Y offset) //
+    ((JZ_len+ZERO_len+JMP_len+INC_len) + offset, w) ->>
+    (UNPACK_len + offset, vec_change (vec_change (vec_change w X n) Y (m+vec_pos w Y)) A 0).
+  { move=> H. apply: sss_compute_trans. { apply: H. by rewrite !(vec_norm HXY). }
+    apply: sss_compute_refl'. congr pair. by rewrite !(vec_norm HXY) Nat.add_0_r. }
+  elim: m {H'X}.
+  { move=> w H'X.
+    apply: (compose_sss_compute_trans 4). { by apply: HALF_spec. }
+    rewrite H'X half_spec_odd Nat.add_0_l !(vec_norm HXY).
+    by apply: sss_compute_refl. }
+  move=> m IH w H'X.
+  apply: (compose_sss_compute_trans 4). { by apply: HALF_spec. }
+  rewrite H'X half_spec_even.
+  apply: (compose_sss_compute_trans 3). { by apply: INC_spec. }
+  apply: sss_compute_trans. { apply: IH. by rewrite !(vec_norm HXY) !(vec_norm HX). }
+  apply: sss_compute_refl'. congr pair.
+  do ? rewrite ?(vec_norm HXY) ?(vec_norm HX) ?(vec_norm HY).
+  by rewrite Nat.add_succ_comm.
+Qed.
+
+Lemma UNPACK0_spec {A X Y v offset} :
+  vec_pos v X = 0 ->
+  (offset, UNPACK A X Y offset) // (offset, v) ->> (0, v).
+Proof.
+  move=> H'X.
+  apply: (compose_sss_compute_trans 0). { by apply: JZ_spec. }
+  rewrite H'X. by apply: sss_compute_refl.
+Qed.
+
+End FixCounters.
