theories/Shared/Libs/DLW/Vec/pos.v
@@ -287,6 +287,13 @@ Proof.
   rewrite map_length; f_equal; auto.
 Qed.
 
+Fact pos_list_NoDup n : NoDup (pos_list n).
+Proof.
+  induction n as [|n IH]; simpl; constructor.
+  - now intros [? [? ?]]%in_map_iff.
+  - apply (FinFun.Injective_map_NoDup (@pos_nxt_inj n) IH).
+Qed.
+
 Section pos_map.
 
   Definition pos_map m n := pos m -> pos n.
