theories/Shared/deterministic_simulation.v
@@ -30,50 +30,66 @@ Section Preliminaries.
     intros ? [u [??]]. exists u. eauto using clos_refl_trans.
   Qed.
 
+  Lemma clos_trans_clos_refl_trans s t : clos_trans _ step s t -> clos_refl_trans _ step s t.
+  Proof.
+    intros H. now induction H; eauto using clos_refl_trans.
+  Qed.
+
 End Preliminaries.
 
 Section Deterministic_simulation.
 
   (* configuration spaces *)
-  Variable (X Y : Type).
+  Context {X Y : Type}.
 
   (* step functions *)
-  Variables (step1 : X -> X -> Prop) (step2 : Y -> Y -> Prop).
+  Context {step1 : X -> X -> Prop} {step2 : Y -> Y -> Prop}.
 
   (* configuration encoding *)
-  Variable (sync : X -> Y -> Prop).
+  Context {sync : X -> Y -> Prop}.
 
   (* determinism of step2 *)
-  Variable (step2_det : forall s' t1' t2', step2 s' t1' -> step2 s' t2' -> t1' = t2').
+  Context (step2_det : forall s' t1' t2', step2 s' t1' -> step2 s' t2' -> t1' = t2').
   Arguments step2_det {s' t1' t2'}.
 
   (* step simulation wrt. encoding *)
-  Variable (fstep : forall s t s', step1 s t -> sync s s' ->
+  Context (fstep : forall s t s', step1 s t -> sync s s' ->
                      exists t', clos_trans Y step2 s' t' /\ sync t t').
   Arguments fstep {s t s'}.
 
   (* halting simulation wrt. encoding *)
-  Variable (fstop : forall s s', stuck step1 s -> sync s s' -> terminates step2 s').
+  Context (fstop : forall s s', stuck step1 s -> sync s s' -> terminates step2 s').
+  Arguments fstop {s s'}.
 
   (* propositional progress/halting decision *)
-  Variable (step1_intro : forall s, (exists t, step1 s t) \/ stuck step1 s).
+  Context (step1_intro : forall s, (exists t, step1 s t) \/ stuck step1 s).
 
-  (* transport of termination by structural induction on transitive closure *)
-  Lemma terminates_transport s s' :
+  (* transport of reachability by structural induction on transitive closure *)
+  Lemma clos_refl_trans_transport {s s' t} :
+    sync s s' -> clos_refl_trans _ step1 s t ->
+    exists t', sync t t' /\ clos_refl_trans _ step2 s' t'.
+  Proof using fstep.
+    intros Hss' Hst. apply clos_rt_rt1n in Hst.
+    revert s' Hss'. induction Hst as [|??? Hxy Hyz IH].
+    - intros s' ?. exists s'. now split; [|apply rt_refl].
+    - intros s' Hxs'. destruct (fstep Hxy Hxs') as [y' [Hs'y' Hyy']].
+      destruct (IH _ Hyy') as [t' [? Hy't']].
+      exists t'. split; [|eapply rt_trans; [apply clos_trans_clos_refl_trans|]]; eassumption.
+  Qed.
+
+  (* transport of termination by transport of reachability *)
+  Lemma terminates_transport {s s'} :
     sync s s' -> terminates step1 s -> terminates step2 s'.
   Proof using fstop fstep.
-    intros Hss' [t [Hst Ht]]. apply clos_rt_rt1n in Hst.
-    revert s' Hss'. induction Hst as [|??? Hxy Hyz IH].
-    - intros s'. now apply fstop.
-    - intros s' [t' [Hs't' Hyt']]%(fstep Hxy).
-      apply (terminates_extend _ (t := t')).
-      + clear Hyt'. induction Hs't'; eauto using clos_refl_trans.
-      + now apply IH.
+    intros Hss' [t [Hst Ht]].
+    destruct (clos_refl_trans_transport Hss' Hst) as [t' [Htt' Hs't']].
+    apply (terminates_extend _ Hs't').
+    eapply fstop; eassumption.
   Qed.
 
   (* terminating configurations are accessible
      note that (Acc R^-1 s) means s is strongly normalizing for R in a constructive setting *)
-  Lemma terminating_Acc s : terminates step2 s -> Acc (fun y x => step2 x y) s.
+  Lemma terminating_Acc {s} : terminates step2 s -> Acc (fun y x => step2 x y) s.
   Proof using step2_det.
     intros [t [Hst%clos_rt_rt1n Ht]].
     induction Hst as [|??? Hxy Hyz IH]; constructor.
@@ -84,7 +100,7 @@ Section Deterministic_simulation.
   (* reflection of termination by well-founded induction on transitive closure using
      Lemma Acc_clos_trans A R x : Acc R x -> Acc (clos_trans A R) x
      from the Coq standard library *)
-  Lemma terminates_reflection s s' : sync s s' -> terminates step2 s' -> terminates step1 s.
+  Lemma terminates_reflection {s s'} : sync s s' -> terminates step2 s' -> terminates step1 s.
   Proof using step2_det step1_intro fstep.
     intros Hss' Hs'%terminating_Acc%(Acc_clos_trans Y).
     revert s Hss'. induction Hs' as [s' _ IH].
