theories/TM/Reductions/L_computable_to_TM_computable.v
@@ -1,3 +1,20 @@
+From Undecidability Require Import
+  MinskyMachines.Reductions.L_computable_to_MMA_computable
+  MinskyMachines.Reductions.MMA_computable_to_MMA_mon_computable
+  TM.Reductions.MMA_mon_computable_to_TM_computable
+  L.L TM.TM.
+
+Lemma L_computable_to_TM_computable k (R : Vector.t nat k -> nat -> Prop) :
+  L_computable R -> TM_computable R.
+Proof.
+  intros H.
+  apply MMA_mon_computable_to_TM_computable.
+  apply MMA_computable_to_MMA_mon_computable.
+  apply L_computable_to_MMA_computable.
+  exact H.
+Qed.
+
+(*
 From Undecidability.TM.L.CompilerBoolFuns Require Import Compiler_spec Compiler_facts Compiler ClosedLAdmissible Compiler_nat_facts.
 
 Lemma L_bool_computable_to_TM_bool_computable k (R : Vector.t (list bool) k -> list bool -> Prop) :
@@ -17,3 +34,4 @@ Proof.
   eapply L_computable_to_L_bool_computable.
   eapply H.
 Qed.
+*)
