theories/TM/Reductions/MMA_computable_to_TM_computable.v
@@ -1,0 +1,13 @@
+From Undecidability Require Import TM.TM MinskyMachines.MMA.
+From Undecidability Require Import
+  MinskyMachines.Reductions.MMA_computable_to_MMA_mon_computable
+  TM.Reductions.MMA_mon_computable_to_TM_computable.
+
+Theorem MMA_computable_to_TM_computable k (R : Vector.t nat k -> nat -> Prop) :
+  MMA_computable R -> TM_computable R.
+Proof.
+  intros H.
+  apply MMA_mon_computable_to_TM_computable.
+  apply MMA_computable_to_MMA_mon_computable.
+  apply H.
+Qed.
